Peano Addition

MathLogic/FOL/Deduction/Equality.lean
@@ -1,7 +1,7 @@
 import MathLogic.FOL.Syntax
 import MathLogic.FOL.Deduction.Minimal
 
-class EqualityDeduction (S : Signature) (α : Type) [BEq α] [MinimalFOLDeduction S α] (eq_pred : S.Pred) where
+class EqualityDeduction (S : Signature) (α : Type) [BEq α] [MinimalFOLDeduction S α] (eq_pred : outParam S.Pred) where
   refl : ∀ (t : Term S α),
     ⊢ .pred eq_pred [t, t]
 
